new/proof/std.v
@@ -8,12 +8,17 @@ Context `{hG: heapGS Σ, !ffi_semantics _ _}.
 Context `{!goGlobalsGS Σ}.
 Context `{!std.GlobalAddrs}.
 
+Definition is_initialized : iProp Σ :=
+  "#?" ∷ std.is_defined ∗
+  "#?" ∷ primitive.is_defined.
+
 Lemma wp_SumNoOverflow (x y : u64) :
-  {{{ std.is_defined }}}
+  {{{ is_initialized }}}
     func_call #std.pkg_name' #"SumNoOverflow" #x #y
   {{{ RET #(bool_decide (uint.Z (word.add x y) = (uint.Z x + uint.Z y)%Z)); True }}}.
 Proof.
-  iIntros (Φ) "#Hdef HΦ".
+  iIntros (Φ) "#Hi HΦ".
+  iNamed "Hi".
   wp_func_call.
   wp_call.
   wp_alloc y_ptr as "Hy".
@@ -31,18 +36,18 @@ Proof.
 Qed.
 
 Lemma wp_SumAssumeNoOverflow (x y : u64) :
-  {{{ std.is_defined }}}
+  {{{ is_initialized }}}
     func_call #std.pkg_name' #"SumAssumeNoOverflow" #x #y
   {{{ RET #(word.add x y); ⌜uint.Z (word.add x y) = (uint.Z x + uint.Z y)%Z⌝ }}}.
 Proof.
-  iIntros "* #Hdef HΦ". wp_func_call. wp_call.
+  iIntros "* #Hi HΦ". iNamed "Hi". wp_func_call. wp_call.
   wp_alloc y_ptr as "Hy".
   wp_pures.
   wp_alloc x_ptr as "Hx".
   wp_pures. wp_load. wp_pures. wp_load.
   wp_pures. wp_apply (wp_SumNoOverflow with "[$]").
   wp_pures.
-  wp_apply wp_Assume.
+  wp_apply (wp_Assume with "[$]").
   rewrite bool_decide_eq_true.
   iIntros (?). wp_pures. do 2 wp_load. wp_pures.
   iApply "HΦ". iPureIntro. done.
